compose/ModTuple2.v
@@ -1,0 +1,205 @@
+Require Import Events.
+Require Import Values.
+Require Import AST.
+Require Import Memory.
+Require Import Globalenvs.
+Require Import Smallstep.
+Require Import CoqlibC.
+Require Import Skeleton.
+Require Import Integers.
+Require Import ASTC.
+Require Import Maps.
+Require Import AxiomsC.
+
+Require Import Mod Sem ModSem.
+Require Import Any.
+
+Set Implicit Arguments.
+
+
+
+
+
+
+
+
+
+
+
+
+Section ANY.
+
+Polymorphic Inductive Any: Type :=
+  Any_intro : forall {A:Type} {x:A}, Any.
+
+(* Arguments Any [A P]. *)
+
+
+Section UNIV.
+Polymorphic Universe i.
+Polymorphic Definition upcast {T: Type@{i}} (a: T): Any := @Any_intro _ a.
+End UNIV.
+
+Section UNIV.
+  
+Polymorphic Universe i j.
+Polymorphic Definition downcast (T: Type@{j}) (a: Any@{i}): option T.
+(* Polymorphic Definition downcast (a: Any) (T: Type): option T. *)
+destruct a.
+destruct (ClassicalDescription.excluded_middle_informative (A = T)).
+- subst. apply Some. assumption.
+- apply None.
+Defined.
+
+Require Import Program.
+
+Polymorphic Lemma upcast_downcast
+      T (a: T)
+  :
+    downcast T (upcast a) = Some a
+.
+Proof.
+  ss. des_ifs. dependent destruction e. ss.
+Qed.
+
+End UNIV.
+
+
+End ANY.
+
+Arguments Any_intro {A} x.
+Global Opaque downcast upcast.
+Print downcast.
+Print upcast.
+Print Any.
+
+
+
+
+
+
+
+
+
+
+
+
+
+Lemma nth_error_nth
+      X
+      (xs: list X) n x
+      (NTH: nth_error xs n = Some x)
+  :
+    forall d, nth n xs d = x
+.
+Proof.
+  ginduction xs; ii; ss; des_ifs; ss; clarify.
+  exploit IHxs; eauto.
+Qed.
+
+Local Obligation Tactic := idtac.
+
+Variable ms_bot: ModSem.t.
+
+Module ModSem2.
+
+  Variable mss: list ModSem.t.
+
+  Record owned_heap: Type := mk_oh3 {
+    anys: list Any;
+    (* OHWTY: forall *)
+    (*     n any *)
+    (*     (NTHA: nth_error anys n = Some any) *)
+    (*   , *)
+    (*     exists elem, (<<CAST: @downcast (nth n mss ms_bot).(ModSem.owned_heap) any = Some elem>>) *)
+    (* ; *)
+  }
+  .
+  Print Universes.
+  (* ModSem.t.u1 <= owned_heap.u0). *)
+  
+  Program Definition initial_owned_heap: owned_heap :=
+    @mk_oh3
+      (map (fun ms => upcast (ModSem.initial_owned_heap ms)) mss)
+      (* _ *)
+  .
+  Print Universes.
+  (* Next Obligation. *)
+  (*   i. rewrite list_map_nth in *. unfold option_map in *. des_ifs. *)
+  (*   erewrite nth_error_nth; eauto. *)
+  (*   esplits; eauto. *)
+  (*   rewrite upcast_downcast. et. *)
+  (* Qed. *)
+
+  Definition genvtype: Type := unit.
+
+  Set Printing Universes.
+
+  Inductive state: Type :=
+  | StateNil
+  | StateCons
+      n
+      (* (st0: (nth n (map (ModSem.state) mss) Empty_set)) *)
+      (st0: (nth n mss ms_bot).(ModSem.state))
+      (tl: state)
+  .
+
+  Inductive find_fptr_owner (fptr: val) (ms: ModSem.t): Prop :=
+  | find_fptr_owner_intro
+      (MODSEM: In ms mss)
+      if_sig
+      (INTERNAL: Genv.find_funct ms.(ModSem.skenv) fptr = Some (Internal if_sig)).
+
+  Inductive step (se: Senv.t) (ge: genvtype): state -> trace -> state -> Prop :=
+  | step_internal
+      n st0 tr st1 tl
+      (STEP: Step (nth n mss ms_bot) st0 tr st1)
+    :
+      step se ge (StateCons n st0 tl)
+           tr (StateCons n st1 tl)
+  .
+
+  (* Inductive step' (se: Senv.t) (ge: genvtype) (st0: state) (tr: trace) (st1: state): Prop := *)
+  (* | step'_internal *)
+  (*     n *)
+  (*     (NTH: match (nth_error mss n) with *)
+  (*           | Some ms => *)
+  (*             exists (hd0 hd1: ms.(ModSem.state)), *)
+  (*               <<STK0: hd_error (get_stk st0) = Some (upcast (n, hd0))>> /\ *)
+  (*               (* <<STK0: hd_error (get_stk st0) = Some (upcast (n, hd0))>> /\ *) *)
+  (*               (* <<STK1: hd_error (get_stk st1) = Some (upcast (n, hd1))>> /\ *) *)
+  (*               <<OH: get_ohs st0 = get_ohs st1>> /\ *)
+  (*               <<STEP: Step ms hd0 tr hd1>> *)
+  (*           | _ => False *)
+  (*           end *)
+  (*     ) *)
+  (* . *)
+  (* Reset step'. *)
+
+  (* Print Universes. *)
+
+  Variable skenv_link: SkEnv.t.
+
+  Variable link_skenv: SkEnv.t -> SkEnv.t -> SkEnv.t.
+
+  Set Printing Universes.
+  Print Universes.
+
+  Program Definition t': ModSem.t :=
+    {|
+      ModSem.state := state;
+      ModSem.owned_heap := owned_heap;
+      ModSem.genvtype := genvtype;
+      (* ModSem.step := step; *)
+      (* ModSem.at_external := coerce at_external; *)
+      (* ModSem.initial_frame := coerce initial_frame; *)
+      (* ModSem.final_frame := coerce final_frame; *)
+      (* ModSem.after_external := ms0.(ModSem.after_external); *)
+      (* ModSem.globalenv := ge; *)
+      (* ModSem.skenv := link_skenv ms0.(ModSem.skenv) ms1.(ModSem.skenv); *)
+      (* ModSem.skenv_link := skenv_link; *)
+      (* ModSem.midx := None; *)
+    |}
+  .
+
+End ModSem2.
